share/pulse/examples/dice/dpe/SPDM3.fst
@@ -1,0 +1,392 @@
+module SPDM3
+
+open Pulse.Lib.Pervasives
+open PulseCore.Preorder
+
+module G = FStar.Ghost
+module U32 = FStar.UInt32
+
+module V = Pulse.Lib.Vec
+module FP = Pulse.Lib.PCM.FractionalPreorder
+module L = FStar.List.Tot
+
+
+type u8 = FStar.UInt8.t
+type u16 = FStar.UInt16.t
+type u32 = FStar.UInt32.t
+
+type u8_v = FStar.UInt8.v
+type u16_v = FStar.UInt16.v
+type u32_v = FStar.UInt32.v
+
+//
+// Setup:
+// We will call a (possible empty) sequence of no_sign_resp messages, followed by a
+//   sign_resp_message as a session
+//
+
+//
+// Concrete state
+// Only maintains the current session transcript
+// This is the memory state associated with a state of the state machine. A state of the state machine takes
+// the current memory state and returns a state of the state machine.
+//
+noeq
+type st = {
+  key_size : u32;
+  signing_pub_key : V.vec u8;
+  session_transcript : V.vec u8;
+}
+
+type g_transcript = (Seq.seq u8)
+
+// Ghost repr
+//
+noeq
+type repr = {
+  signing_pub_key_repr : Seq.seq u8;
+  transcript : g_transcript;
+}
+
+let g_transcript_non_empty (t:g_transcript) : prop =
+  Seq.length t > 0
+
+let is_initialized_transcript (t:g_transcript) : prop =
+  Seq.equal t Seq.empty
+
+//
+// States of the state machine
+//
+noeq
+type state =
+  | Initialized : st -> state
+  | Recv_no_sign_resp : st -> state
+
+//
+// Corresponding ghost states
+//
+noeq
+type g_state : Type u#1 =
+  | G_UnInitialized : g_state
+  | G_Initialized : repr:repr{is_initialized_transcript repr.transcript} -> g_state
+  | G_Recv_no_sign_resp : repr:repr ->  g_state
+
+  | G_Recv_sign_resp : repr:repr -> g_state
+
+let is_prefix_of (#a:Type) (s0 s1:Seq.seq a) : prop =
+  Seq.length s0 < Seq.length s1 /\
+  s0 == Seq.slice s1 0 (Seq.length s0)
+
+  //
+// The transition function
+//
+let next (s0 s1:g_state) : prop =
+  match s0, s1 with
+  //Uninit ---> initial (upon init call)
+  |G_UnInitialized, G_Initialized r -> true
+  //initial ---> no_sign (upon no_sign call)
+  | G_Initialized r0 , G_Recv_no_sign_resp r1 ->
+        g_transcript_non_empty r1.transcript
+
+  // initial ---> sign (upon sign call)
+  | G_Initialized r0 , G_Recv_sign_resp r1->
+        g_transcript_non_empty r1.transcript
+
+  // no_sign --> no_sign (upon no_sign call)
+  | G_Recv_no_sign_resp r0 ,  G_Recv_no_sign_resp r1 ->
+        g_transcript_non_empty r1.transcript /\
+        g_transcript_non_empty r0.transcript /\
+        is_prefix_of r0.transcript r1.transcript
+
+  //no_sign ---> sign (upon sign call)
+  | G_Recv_no_sign_resp r0, G_Recv_sign_resp r1  ->
+        g_transcript_non_empty r1.transcript /\
+        g_transcript_non_empty r0.transcript /\
+        is_prefix_of r0.transcript r1.transcript
+        
+  //sign ---> initial (no call is needed)
+  | G_Recv_sign_resp r0, G_Initialized r1 ->
+        g_transcript_non_empty r0.transcript 
+
+  //no_sign --> initial (upon reset call)
+  |G_Recv_no_sign_resp r0, G_Initialized r1 ->
+        g_transcript_non_empty r0.transcript
+
+  | _ -> False
+
+//
+// Until gref, this is setting up the trace PCM
+//
+noextract
+let rec well_formed_trace (l:list g_state) : prop =
+  match l with
+  | []
+  | [G_Initialized _] -> True
+  | s1::s0::tl -> next s0 s1 /\ well_formed_trace (s0::tl)
+  | _ -> False
+
+noextract
+type trace_elt : Type u#1 = l:list g_state { well_formed_trace l }
+
+noextract
+let trace_extension (t0 t1:trace_elt) : prop =
+  Cons? t1 /\ t0 == List.Tot.tail t1
+
+noextract
+let trace_preorder : FStar.Preorder.preorder trace_elt =
+  FStar.ReflexiveTransitiveClosure.closure trace_extension
+
+noextract
+type trace = hist trace_preorder
+
+noextract
+type trace_pcm_t : Type u#1 = FP.pcm_carrier trace_preorder
+
+noextract
+let trace_pcm : FStar.PCM.pcm trace_pcm_t = FP.fp_pcm trace_preorder
+
+noextract
+let current_state (t:trace) : g_state =
+  match t with
+  | [] -> G_UnInitialized
+  | hd::_ ->
+    match hd with
+    | [] -> G_UnInitialized
+    | s::_ -> s
+
+noextract
+let valid_transition (t:trace) (s:g_state) : prop =
+  next (current_state t) s
+
+noextract
+let next_trace (t:trace) (s:g_state { valid_transition t s }) : trace =
+  match t with
+  | [] -> [[s]]
+  | hd::tl ->
+    match hd with
+    | [] -> [s]::t
+    | l -> (s::l)::t
+
+noextract
+type gref = ghost_pcm_ref trace_pcm
+
+let session_state_related (s:state) (gs:g_state) : v:slprop { is_slprop2 v } =
+  match s, gs with
+  | Initialized st, G_Initialized repr
+  | Recv_no_sign_resp st, G_Recv_no_sign_resp repr ->
+    V.pts_to st.signing_pub_key repr.signing_pub_key_repr **
+    V.pts_to st.session_transcript repr.transcript
+
+  | _ -> pure False
+
+  //
+// The main invariant
+// The session_state_related connects the concrete state with the current ghost state of the trace.
+// r is the trace pointer with permission
+//
+let inv (s:state) (r:gref) (t:trace) : v:slprop { is_slprop2 v } =
+  ghost_pcm_pts_to r (Some 1.0R, t) **
+  session_state_related s (current_state t)
+
+assume val trace_ref : gref
+
+let init_client_perm (s:state) : slprop =
+  exists* (t:trace).
+    inv s trace_ref t ** pure (G_Initialized? (current_state t))
+
+assume val init (key_len:u32) (signing_key:V.vec u8 { V.length signing_key == U32.v key_len })
+  : stt state (requires exists* p b. V.pts_to signing_key #p b)
+              (ensures fun s -> exists* p b. V.pts_to signing_key #p b ** init_client_perm s)
+
+
+noeq
+type resp_repr = {
+  some_field : u32;
+  // TODO
+}
+
+//
+// Related to parser
+//
+assume val valid_resp (resp:V.vec u8) (repr:resp_repr) : slprop
+
+type result =
+  | Success
+  | Parse_error
+  | Signature_verification_error
+
+//
+//Measurement block structure
+//
+
+noeq
+type spdm_measurement_block_t  = {
+  index : u8;
+  measurement_specification : u8;
+  measurement_size : u16;
+  measurement : V.vec u8
+}
+//
+//result structure
+//
+noeq
+type spdm_measurement_result_t  = {
+  measurement_block_vector : V.vec  spdm_measurement_block_t;
+  measurement_block_count : u8;
+  status : result
+}
+
+//
+//Signature of get_measurement_blocks_without_signature
+//
+let valid_state (s:g_state) :prop =
+  G_Initialized? s \/ G_Recv_no_sign_resp? s \/ G_Recv_sign_resp? s
+
+let g_transcript_of_gst (s:g_state { valid_state s })
+  : g_transcript =
+  match s with
+  | G_Initialized r
+  | G_Recv_no_sign_resp r
+  | G_Recv_sign_resp r -> r.transcript
+
+let g_key_of_gst (s:g_state { valid_state s })
+  : Seq.seq u8 =
+  match s with
+  | G_Initialized r
+  | G_Recv_no_sign_resp r
+  | G_Recv_sign_resp r -> r.signing_pub_key_repr
+
+let current_transcript (t:trace { valid_state (current_state t) }) : g_transcript =
+  g_transcript_of_gst (current_state t)
+
+let current_key (t:trace { valid_state (current_state t) }) : Seq.seq u8 =
+  g_key_of_gst (current_state t)
+
+let g_transcript_current_session_grows (t0 t1:g_transcript) : prop =
+  is_prefix_of t0 t1 
+
+let g_transcript_current_session_grows_by (t0 t1:g_transcript) (s:Seq.seq u8) : prop =
+   g_transcript_current_session_grows t0 t1 /\
+   t1 == Seq.append t0 s
+
+let g_transcript_current_session_grows_lemma (t0 t1:g_transcript) (s:Seq.seq u8)
+  : Lemma (g_transcript_current_session_grows_by t0 t1 s ==>
+           g_transcript_current_session_grows t0 t1) = ()
+
+
+assume val no_sign_resp
+  (req:V.vec u8)
+  (resp:V.vec u8)
+  (req_size: u8)
+  (resp_size: u8)
+  (st:state)
+  (#tr0:trace {valid_state (current_state tr0) })
+  : stt spdm_measurement_result_t 
+    (requires (exists* p_req b_req p_resp b_resp.
+                          V.pts_to req #p_req b_req **
+                          V.pts_to resp #p_resp b_resp **
+                          pure (Seq.length b_req == u8_v req_size) **
+                          pure (Seq.length b_resp == u8_v resp_size)) **
+                          inv st trace_ref tr0 **
+                          pure (G_Recv_no_sign_resp? (current_state tr0) \/
+                                G_Initialized? (current_state tr0))
+                          )
+    (ensures fun res -> 
+               (exists* p_req b_req p_resp b_resp.
+                         V.pts_to req #p_req b_req **
+                         V.pts_to resp #p_resp b_resp **
+                         pure (Seq.length b_req == u8_v req_size) **
+                         pure (Seq.length b_resp == u8_v resp_size) **
+                         (let measurement_blocks = res.measurement_block_vector in
+                          let measurement_block_count = res.measurement_block_count in
+                          let result = res.status in
+                          (match result with
+                          | Parse_error -> pure (u8_v measurement_block_count == 0) //zero out the measurement blocks
+                          | Signature_verification_error -> pure False
+                          | Success -> 
+                               (exists* r tr1. valid_resp resp r **
+                                        inv st trace_ref tr1 **
+                                        (let s = current_state tr1 in
+                                        pure (G_Recv_no_sign_resp? s) **
+                                        pure (valid_transition tr0 s) **
+                                        pure (valid_transition tr0 s /\ tr1 == next_trace tr0 s)
+                                        ) **
+                                        (let t0 = current_transcript tr0 in
+                                         let t1 = current_transcript tr1 in
+                                         pure (g_transcript_current_session_grows_by t0 t1 (Seq.append b_req b_resp)))
+                                )))))
+
+assume val valid_signature (signature msg key:Seq.seq u8): prop
+
+assume val sign_resp
+  (req:V.vec u8)
+  (resp:V.vec u8)
+  (req_size: u8)
+  (resp_size: u8)
+  (st:state)
+  (#tr0:trace {valid_state (current_state tr0) })
+  : stt spdm_measurement_result_t 
+    (requires (exists* p_req b_req p_resp b_resp.
+                          V.pts_to req #p_req b_req **
+                          V.pts_to resp #p_resp b_resp **
+                          pure (Seq.length b_req == u8_v req_size) **
+                          pure (Seq.length b_resp == u8_v resp_size)) **
+                          inv st trace_ref tr0 **
+                          pure (G_Recv_no_sign_resp? (current_state tr0) \/
+                                G_Initialized? (current_state tr0))
+                          )
+    (ensures fun res -> 
+               (exists* p_req b_req p_resp b_resp.
+                         V.pts_to req #p_req b_req **
+                         V.pts_to resp #p_resp b_resp **
+                         pure (Seq.length b_req == u8_v req_size) **
+                         pure (Seq.length b_resp == u8_v resp_size) **
+                         (let measurement_blocks = res.measurement_block_vector in
+                          let measurement_block_count = res.measurement_block_count in
+                          let result = res.status in
+                          
+                          (match result with
+                          | Parse_error -> pure (u8_v measurement_block_count == 0) //zero out the measurement blocks
+                          | Signature_verification_error -> pure (u8_v measurement_block_count == 0)
+                          | Success -> 
+                               (exists* r tr1 sign inter_gstate inter_trace. valid_resp resp r **
+                                        inv st trace_ref tr1 **
+                                        //tr1 current_state is G_Initailized
+                                        pure (G_Initialized? (current_state tr1)) **
+                                        //intermedite trace inter_trace exists and inter g_state exists
+                                        pure (G_Recv_sign_resp?inter_gstate) **
+                                        //Relation between inter_trace and inter_gstate
+                                        pure (current_state inter_trace == inter_gstate) **
+
+                                        //inter_trace transcript gets the req resp appended
+                                        (let s = current_state tr1 in
+                                         let s1 = current_state inter_trace in
+                                         let t0 = current_transcript tr0 in
+                                         let t' = current_transcript inter_trace in
+                                         let key = current_key inter_trace in
+                                         let msg = t' in
+
+                                         //From inter_trace l2 is found out
+                                         pure (valid_signature sign msg key) **
+                                         pure (g_transcript_current_session_grows_by t0 t' (Seq.append b_req b_resp)) **
+                                         pure (valid_transition tr0 s1 /\ 
+                                                valid_transition inter_trace s)) **
+                                        
+                                        //inter_trace ---> tr1
+                                        (let t1 = current_transcript tr1 in
+                                         pure (t1 == Seq.empty)
+                                         )
+                                )))))
+
+//
+//Reset function
+//
+assume val reset
+  (st:state)
+  (#tr0:trace {valid_state (current_state tr0) })
+  : stt unit
+    (requires (inv st trace_ref tr0 **
+                          pure (G_Recv_no_sign_resp? (current_state tr0))
+                          ))
+    (ensures fun res -> init_client_perm st)
+
